Observe that $a=b\cos C+c\cos B$ and cyclic expressions, so summing this up gives \[a+b+c=\left(b+c\right)\cos A+\left(c+a\right)\cos B+\left(a+b\right)\cos C.\] Now, observe that $\left[BOC\right]=\frac{aR\cos A}{2}$ and cyclic expressions, so \[\frac{r\left(a+b+c\right)}{R}=\frac{2\left[ABC\right]}{R}=a\cos A+b\cos B+c\cos C.\] Adding these two equations together gives that \[\left(a+b+c\right)\left(1+\frac{r}{R}\right)=\left(a+b+c\right)\left(\cos A+\cos B+\cos C\right),\] from which the equality follows.