Consider the polynomial \[P\left(x\right)=\displaystyle\sum_{i=1}^5a_i\displaystyle\prod_{\substack{0\leq j\leq5\\j\neq i}}\left(x+j\right)-\left(x+1\right)\left(x+2\right)\cdots\left(x+5\right).\] By plugging in $k^2$ for $k=2,3,4,5,6$, we see that these are all roots of $P$, so there is some constant $C$ such that \[P\left(x\right)=C\left(x-4\right)\left(x-9\right)\left(x-16\right)\left(x-25\right)\left(x-36\right).\] Now, observe that \[-\left(6!\right)^2C=P\left(0\right)=-5!\] because all of the terms of the summation in $P$ have a factor of $x$, so $C=\frac{1}{6\cdot6!}$. Then \[P\left(1\right)=-\frac{1}{6\cdot6!}\displaystyle\prod_{k=2}^6\left(k^2-1\right)=\frac{7!}{2\cdot6^2}.\] But observe that \[\frac{P\left(1\right)}{6!}+1=\frac{a_1}{2}+\frac{a_2}{3}+\frac{a_3}{4}+\frac{a_4}{5}+\frac{a_5}{6},\] so the requested sum is $1-\frac{7}{2\cdot6^2}=\boxed{\frac{65}{72}}$.