This is an exercise in PIE with casework. Let $A$ be the sum over all triples of smooth numbers, $B$ be the sum over all triples with $\gcd\left(a,b\right)=\gcd\left(a,c\right)$, and $C$ be the sum over all triples with $\gcd\left(b,c\right)=\gcd\left(c,a\right)=\gcd\left(a,b\right)$. The sum $A-3B+2C$ counts each triple in $S$ exactly once, each triple with $\gcd\left(a,b\right)=\gcd\left(a,c\right)\neq\gcd\left(b,c\right)$ (as well as symmetric types) no times, and each triple with $\gcd\left(b,c\right)=\gcd\left(c,a\right)=\gcd\left(a,b\right)$ no times, hence this is the value we wish to compute.

To shorthand, let $a=2^{m_a}3^{n_a},b=2^{m_b}3^{n_b},c=2^{m_c}3^{n_c}$.

To compute $A$, observe that the sum is \[\displaystyle\sum_{m_a,m_b,m_c,n_a,n_b,n_c\geq0}\frac{1}{2^{m_a+m_b+m_c}3^{n_a+n_b+n_c}}\]\[=\left(\displaystyle\sum_{m\geq0}\frac{1}{2^m}\right)^3\left(\displaystyle\sum_{n\geq0}\frac{1}{3^n}\right)^3=\frac{2^3}{\left(2-1\right)^3}\cdot\frac{3^3}{\left(3-1\right)^3}=27.\]

To compute $B$, consider when $\gcd\left(a,b\right)=\gcd\left(a,c\right)$. If $m_a>m_b$, we need $m_b=m_c$ otherwise $\min\left(m_a,m_c\right)\neq m_b$. If $m_a\leq m_b$, we need $m_c\geq m_a$ so that $\min\left(m_a,m_c\right)=m_a$. Thus, one of $m_a>m_b=m_c$ and $m_a\leq m_a,m_c$ must occur. Similarly, one of $n_a>n_b=n_c$ and $n_a\leq n_b,n_c$ must occur. Furthermore, these parts are independent, so we can factor the sum into separate sums for $2$ and $3$ as any working inequality on $m$ can be paired up with any working inequality on $n$. The sum for $2$ is \[\displaystyle\sum_{0\leq m_b<m_a}\frac{1}{2^{m_a+2m_b}}+\displaystyle\sum_{0\leq m_a\leq m_b,m_c}\frac{1}{2^{m_a+m_b+m_c}}\]\[=\displaystyle\sum_{m_b,d\geq0}\frac{1}{2^{3m_b+d+1}}+\displaystyle\sum_{m_a,e,f\geq0}\frac{1}{2^{3m_a+d+e}},\] where we set $d=m_a-m_b-1$ in the first sum and $e=m_b-m_a,f=m_c-m_a$ in the second sum. This evaluates to \[\frac{2^3}{2^3-1}\cdot\frac{2}{2-1}\cdot\frac{1}{2}+\frac{2^3}{2^3-1}\cdot\frac{2}{2-1}\cdot\frac{2}{2-1}=\frac{40}{7}.\] Similarly, the sum for $3$ evaluates to \[\frac{3^3}{3^3-1}\cdot\frac{3}{3-1}\cdot\frac{1}{3}+\frac{3^3}{3^3-1}\cdot\frac{3}{3-1}\cdot\frac{3}{3-1}=\frac{297}{104},\] so $B=\frac{40}{7}\cdot\frac{297}{104}=\frac{1485}{91}$.

Finally, we compute $C$. If $m_a>m_b$, we need $m_b=m_c$ in order for $\min\left(m_c,m_a\right)=m_b$. If $m_a=m_b$, we need $m_c\geq m_a$ so that $\min\left(m_c,m_a\right)=\min\left(m_c,m_b\right)=m_a$. If $m_a<m_b$, we need $m_a=m_c$ in order for $\min\left(m_b,m_c\right)=m_a$. Thus, we need one of $m_a>m_b=m_c$, $m_a=m_b\leq m_c$, and $m_a=m_c<m_b$ to happen. We have similar inequalites with $n$. As before, we can factor the sum into the corresponding sums for $2$ and $3$ only. The sum for $2$ is \[\displaystyle\sum_{0\leq m_b<m_a}\frac{1}{2^{m_a+2m_b}}+\displaystyle\sum_{0\leq m_a\leq m_c}\frac{1}{2^{2m_a+m_c}}+\displaystyle\sum_{0\leq m_a<m_b}\frac{1}{2^{2m_a+m_b}}\]\[=\displaystyle\sum_{m_b,d\geq0}\frac{1}{2^{3m_b+d+1}}+\displaystyle\sum_{m_a,e\geq0}\frac{1}{2^{3m_a+e}}+\displaystyle\sum_{m_a,f\geq0}\frac{1}{2^{3m_a+f+1}},\] where we set $d=m_a-m_b-1$ in the first sum, $e=m_c-m_a$ in the second sum, and $f=m_b-m_a-1$ in the third sum. This evaluates to \[\frac{2^3}{2^3-1}\cdot\frac{2}{2-1}\cdot\frac{1}{2}+\frac{2^3}{2^3-1}\cdot\frac{2}{2-1}+\frac{2^3}{2^3-1}\cdot\frac{2}{2-1}\cdot\frac{1}{2}=\frac{32}{7}.\] Similarly, the sum for $3$ evaluates to \[\frac{3^3}{3^3-1}\cdot\frac{3}{3-1}\cdot\frac{1}{3}+\frac{3^3}{3^3-1}\cdot\frac{3}{3-1}+\frac{3^3}{3^3-1}\cdot\frac{3}{3-1}\cdot\frac{1}{3}=\frac{135}{52},\] so $C=\frac{32}{7}\cdot\frac{135}{52}=\frac{1080}{91}$.

Hence the sum we are looking for is \[A-3B+2C=27-3\cdot\frac{1485}{91}+2\cdot\frac{1080}{91}=\boxed{\frac{162}{91}}.\]