Write
\[
	\frac{\sin\frac{(2k-1)\pi}{2n}}{\cos^2\frac{(k-1)\pi}{2n}\cos^2\frac{k\pi}{2n}}=\frac{4\sin\frac{(2k-1)\pi}{2n}}{\left(1+\cos\frac{2(k-1)\pi}{2n}\right)\left(1+\cos\frac{2k\pi}{2n}\right)}=-\frac{2}{\sin\frac{\pi}{2n}}\left(\frac{1}{1+\cos\frac{2(k-1)\pi}{2n}}-\frac{1}{1+\cos\frac{2k\pi}{2n}}\right)
\]
by half-angle then sum-to-product. So
\[
	a_n=\sum_{k=1}^{n-1}\frac{\sin\frac{(2k-1)\pi}{2n}}{\cos^2\frac{(k-1)\pi}{2n}\cos^2\frac{k\pi}{2n}}=-\frac{2}{\sin\frac{\pi}{2n}}\left(\frac{1}{2}-\frac{1}{1+\cos\frac{2(n-1)\pi}{2n}}\right)=-\frac{2}{\sin\frac{\pi}{2n}}\left(\frac{1}{2}-\frac{1}{2\sin^2\frac{\pi}{2n}}\right).
\]
Since $\sin\frac{\pi}{2n}=\frac{\pi}{2n}+O(n^{-3})$ by Taylor expansion, 
\[
	a_n=-\frac{2}{\frac{\pi}{2n}+O(n^{-3})}\left(\frac{1}{2}-\frac{1}{\frac{\pi^2}{2n^2}+O(n^{-4})}\right)=n^3\left(\frac{8}{\pi^3+O(n^{-2})}-\frac{2}{\pi n^2+O(1)}\right)
\]
whence $\ds\lim_{n\to\infty}\frac{a_n}{n^3}=\boxed{\frac{8}{\pi^3}}$ as desired.