The condition $IG\parallel AB$ is equivalent to $\frac{r}{h_C}=\frac{1}{3}$, which (using $K=rs=\frac{ch_C}{2}$) implies that $a+b=2c$. So $\sin\alpha+\sin\beta=2\sin\gamma$ where $\gamma=\angle{C}$.

Let $x=e^{i\alpha},y=e^{i\beta},z=e^{i\gamma}$ so that $xyz=-1$. Then
\[
	\frac{x-x^{-1}}{2i}+\frac{y-y^{-1}}{2i}=\frac{z-z^{-1}}{i}
\]
so
\[
	(2y-1)x-(y-y^{-1})+(1-2y^{-1})x^{-1}=0.
\]
With $y=\frac{(3+i)^2}{10}=\frac{4}{5}+i\frac{3}{5}$, this gives
\[
	\left(x-i\right)\left(\left(\frac{3}{5}+i\frac{6}{5}\right)-\left(\frac{6}{5}+i\frac{3}{5}\right)\right)=\left(\frac{3}{5}+i\frac{6}{5}\right)x-i\frac{6}{5}+\left(-\frac{3}{5}+i\frac{6}{5}\right)x^{-1}=0
\]
so $x=i$ and thus $\alpha=\boxed{\frac{\pi}{2}}$.