Let $b_i$, $1\leq i\leq n-1$, be the $i$th smallest member of \[S=\left\{a_j-a_i\mid i\leq i<j\leq n\right\}.\] I claim that $a_k-a_2$ and $a_{k-1}-a_1$ are both $b_{k-2}$ for $k=3,4,\ldots,n$. note that \[a_k-a_2<a_{k+1}-a_2<a_{k+2}-a_2<\ldots<a_n-a_2<a_n-a_1,\] so $a_k-a_2$ is less than $n-k+1$ distinct members of $S$. Furthermore, \[a_k-a_2>a_k-a_3>a_k-a_4>\ldots>a_k-a_{k-1},\] so $a_k-a_2$ is greater that $k-3$ distinct members of $S$. These combined give that \[a_k-a_2=b_{k-2}.\] Now, note that \[a_{k-1}-a_1<a_k-a_1<a_{k+1}-a_1<\ldots<a_n-a_2,\] so $a_{k-1}-a_1$ is less than $n-k+1$ distinct members of $S$. Furthermore, \[a_{k-1}-a_1>a_{k-1}-a_2>a_{k-1}-a_3>\ldots>a_{k-1}-a_{k-2},\] so $a_{k-1}-a_1$ is greater than $k-3$ distinct members of $S$. These combined give that \[a_{k-1}-a_1=b_{k-2},\] so the claim is proven. But then \[a_k=a_{k-1}+\left(a_2-a_1\right),\] so $a_1,a_2,\ldots,a_n$ is an arithmetic progression.